coq-minuska/theories/default_everything.v
@@ -20,6 +20,9 @@ Require Export
   Coq.extraction.ExtrOcamlZBigInt
   Coq.extraction.ExtrOcamlNatBigInt
 .
+
+Set Extraction KeepSingleton.
+
 From Coq Require Import String Bool Arith ZArith List.
 
 Require Minuska.BuiltinValue Minuska.builtins.
@@ -35,22 +38,24 @@ Defined.
 
 #[export]
 Instance DSM
-    {β : Builtin MyUnit}
+    {mysignature : Signature}
+    {β : Model MyUnit}
     (program_info : ProgramInfo)
     : StaticModel :=
-    default_model β program_info
+    default_model mysignature β program_info
 .
 
-Definition GT {β : Builtin MyUnit} := @TermOver' string (builtin_value).
+Definition GT {mysignature : Signature} {β : Model MyUnit} := @TermOver' string (builtin_value).
 
-Definition StepT {β : Builtin MyUnit} (program_info : ProgramInfo) := ProgramT -> NondetValue -> GT -> option GT.
-Definition StepT_ext {β : Builtin MyUnit} (program_info : ProgramInfo) := ProgramT -> NondetValue -> GT -> option (GT*nat).
+Definition StepT {mysignature : Signature} {β : Model MyUnit} (program_info : ProgramInfo) := ProgramT -> NondetValue -> GT -> option GT.
+Definition StepT_ext {mysignature : Signature} {β : Model MyUnit} (program_info : ProgramInfo) := ProgramT -> NondetValue -> GT -> option (GT*nat).
 
-Definition gt_over {β : Builtin MyUnit} (b : builtin_value) : GT := @t_over string builtin_value b.
-Definition gt_term {β : Builtin MyUnit} (s : string) (l : list GT) : GT := @t_term string builtin_value s l.
+Definition gt_over {mysignature : Signature} {β : Model MyUnit} (b : builtin_value) : GT := @t_over string builtin_value b.
+Definition gt_term {mysignature : Signature} {β : Model MyUnit} (s : string) (l : list GT) : GT := @t_term string builtin_value s l.
 
 Definition basic_rule
-    {β : Builtin MyUnit}
+    {mysignature : Signature}
+    {β : Model MyUnit}
     (program_info : ProgramInfo)
     (name : string)
     (l : TermOver BuiltinOrVar)
@@ -73,7 +78,8 @@ Definition BoV_to_Expr2
 .
 
 Definition framed_rule
-    {β : Builtin MyUnit}
+    {mysignature : Signature}
+    {β : Model MyUnit}
     (program_info : ProgramInfo)
     (frame : (variable*(TermOver BuiltinOrVar)))
     (name : string)
@@ -88,21 +94,24 @@ Definition framed_rule
 .
 
 Definition global_naive_interpreter
-    {β : Builtin MyUnit}
+    {mysignature : Signature}
+    {β : Model MyUnit}
     (program_info : ProgramInfo)
     :=
     @naive_interpreter (DSM program_info) Act
 .
 
 Definition global_naive_interpreter_ext
-    {β : Builtin MyUnit}
+    {mysignature : Signature}
+    {β : Model MyUnit}
     (program_info : ProgramInfo)
     :=
     @naive_interpreter_ext (DSM program_info) Act
 .
 
 Definition global_naive_interpreter_sound
-    {β : Builtin MyUnit}
+    {mysignature : Signature}
+    {β : Model MyUnit}
     (program_info : ProgramInfo)
     :=
     @naive_interpreter_sound (DSM program_info) Act
